#Recursion
- https://leetcode.com/explore/learn/card/recursion-i/250/principle-of-recursion/
##Principle of Recursion
1. A simple base case (or cases) - a terminating scenario that does not use recursion to produce an answer.
2. A set of rules, also known as recurrence relation that reduces all other cases towards the base case.



---

###344. Reverse String
- https://leetcode.com/problems/reverse-string/
- Write a function that reverses a string. The input string is given as an array of characters char[]. 
- Do not allocate extra space for another array, you must do this by modifying the input array in-place with O(1) extra memory. 
- You may assume all the characters consist of printable ascii characters.
```js
Example 1:
Input: ["h","e","l","l","o"]
Output: ["o","l","l","e","h"]

Example 2:
Input: ["H","a","n","n","a","h"]
Output: ["h","a","n","n","a","H"]
```     

```js
/**
 * @param {character[]} s
 * @return {void} Do not return anything, modify s in-place instead.
 */

// 배열의 뒤에서부터 하나씩 추가하고 기존 요소를 삭제
var reverseString = function (s) {
  let count = 0;

  const recursion = function (s) {
    if (count === s.length) return
    let word = s.length - 1
    s.push(s[word - count])
    s.splice(word - count, 1)
    count++
    recursion(s)
  }

  recursion(s)
};
```

```js
// munawiki
var reverseString = function(s) {
  function recursion(s, i, j) {
    if (i >= j) return;
    [s[i], s[j]] = [s[j], s[i]];
    recursion(s, i + 1, j - 1);
  }
  recursion(s, 0, s.length - 1);
  return s;
};
```




---

###24. Swap Nodes in Pairs
- https://leetcode.com/problems/swap-nodes-in-pairs
- Given a linked list, swap every two adjacent nodes and return its head.
- You may not modify the values in the list's nodes. Only nodes itself may be changed.
```js
Example 1:
Input: head = [1,2,3,4]
Output: [2,1,4,3]

Example 2:
Input: head = []
Output: []

Example 3:
Input: head = [1]
Output: [1]

Constraints:
The number of nodes in the list is in the range [0, 100].
0 <= Node.val <= 100
```    
```js
/**
 * Definition for singly-linked list.
 * function ListNode(val, next) {
 *     this.val = (val===undefined ? 0 : val)
 *     this.next = (next===undefined ? null : next)
 * }
 */
/**
 * @param {ListNode} head
 * @return {ListNode}
 */
var swapPairs = function(head) {
    
    const recursion = function(node) {
        if(node === null || node.next === null) return node;
    
        let second  = node.next
        let third = second.next
        // 이 값을 저장해 놓았기 때문에, 2를 1로 가르키게 하고 나서 재귀를 타고
        // 들어갈 때, 1이 3을 가르킬 수 있도록 함 
        second.next = node;
        node.next = recursion(third);
        return second;
    }
    return recursion(head);
};

//    s  t
//          s  t
// 1->2->3->4->Null
// second.next = node; 먼저 2가 1을 가르키게 하고 
// node.next = recursion(third); 1은 재귀의 결과 값을 가르킨다
// recursion(3)이 시작하고 4는 3을 가르키고 3의 next.next인 값인 null이 다시 재귀를 타게 됨
// 탈풀문을 맞이하게 되고 현재 노드는 3이며, 3 ->Null이고 4를 반환
// node.next = recursion(third) => 재귀를 타고 나올 때, 4->3->Null인 상태
// 이 때의 노드는 1이고, 노드의 next를 second라는 변수에 저장해놓았기 때문에
// 2를 반환하게 된다. 2는 이 전에 1을 가르켰고, 1은 재귀에서 나온 4를 가르켰기 때문에
// 2->1->4->3->null인 상태가 된다


```

```js
// 다른 방법
var swapPairs = function(head){
  if(head === null || head.next === null) return head;
  
  const temp = head.next;
  head.next = swapPairs(head.next.next);
  temp.next = head;
  
  return temp;
}
// h  t  h  t
// 1->2->3->4
// head의 다음은 재귀의 결과이고 swapPairs(3)이 들어가게 된다
// 그리고 또 swapPairs(Null)이 들어가니깐 리턴
// temp의 다음은 head임으로 4->3->Null
// head.next => 1의 재귀 결과는 4->3->Null 이고 temp인 2는 head인 1을 가르킨다
// 결국 2->1->4->3->Null이 나온다
```




###Practice how to convert For Loop to RECURSION
- Sum- make a sum of string composed with numbers
- ex. '123'
```js
// console.log(sum('123'))
// for loop
function sum(str) {
  let result = 0
  for (let i = 0; i < str.length; i++) {
    result += Number(str[i])
  }
  return result;
}

// recursion #1
const sum = function (str) {
  if (str.length === 0) return 0
  const head = Number(str[0])
  const tail = str.slice(1)
  return head + sum(tail)
}

// recursion #2
const sum = function(str){
  let result = 0
  const recursion = function(str, i){
    if(i === str.length) return 0;
    result += Number(str[i])
    recursion(str, ++i)
  }
  recursion(str, 0)
  return result;
}
```




---

##Recurrence Relation
- recurrence relation: the relationship between the result of a problem and the result of its subproblems.
- base case: the case where one can compute the answer directly without any further recursion calls. Sometimes, the base cases are also called bottom cases, since they are often the cases where the problem has been reduced to the minimal scale, i.e. the bottom, if we consider that dividing the problem into subproblems is in a top-down manner.

---
###206. Reverse Linked List
- https://leetcode.com/problems/reverse-linked-list/
- Reverse a singly linked list.
```js
Example:
Input: 1->2->3->4->5->NULL
Output: 5->4->3->2->1->NULL

Follow up:
A linked list can be reversed either iteratively or recursively. Could you implement both?

```     

```js
/**
 * Definition for singly-linked list.
 * function ListNode(val, next) {
 *     this.val = (val===undefined ? 0 : val)
 *     this.next = (next===undefined ? null : next)
 * }
 */
/**
 * @param {ListNode} head
 * @return {ListNode}
 */
var reverseList = function(head) {
    let prevPointer = null;
    let currentPointer = head;
    let nextPointer = null;
    
    while(currentPointer !== null){
        nextPointer = currentPointer.next;
        currentPointer.next = prevPointer;
        
        prevPointer= currentPointer;
        currentPointer = nextPointer;
    } 
    
    return prevPointer;
};
// 먼저 cp.next를 변수에 담아준 다음 cp가 오른쪽으로 보던 것을 왼쪽으로 pp를
// 보게 만들기 그리고 나서 pp를 cp의 위치로 옮겨주고, cp는 np의 위치로 옮겨주면서
// 쭉 끝까지 이동을 하게 한다
```


```js
var reverseList = function(head) {
  if(head === null || head.next === null) return head;

  let temp = reverseList(head.next)
  head.next.next = head;
  head.next = null;
  
  return temp
};
// 1->2->3->null
// head: 1 temp = reverseList(2) 3이 반환되고 head인 next인 2는 null이 아니라 이제
// head인 1을 가르키고 head인 1은 null을 가르킨다 3->2->1->null
// head: 2 temp = reverseList(3) 3->null이 재귀를 찍고 나오게 되고 head 2의 다음인 3은
// head를 가르키게 되고 head인 2는 null을 가르킨다 3->2->null
// head: 3 temp = reveseList(null) null을 반환하고 3의 next.next를 head로 가르킨다는데
// null은 아무것도 가르킬 수 없음 3은 null을 가르킨다 3->null

// temp를 마지막으로 반환하니, 반대로 돌린 linkedlist를 반환한다
```

- reference: https://www.geeksforgeeks.org/reverse-a-linked-list/